Earley/Parser.lean
@@ -79,41 +79,57 @@ def toGraphviz [ToString T] [ToString N] (t : Tree T N) : String :=
 /--
 Reconstruct the parse tree by searching the origin data from the EarleyBins.
 TODO: Realistically this should never return none if it gets called with a well-formed bin?
-TODO: termination_by binsIdx obv doesnt work, there should be some sort of well-formed reasoning?
+      termination_by k obv doesnt work, there should be some sort of well-formed reasoning?
 -/
-public partial def buildTree (w : List T) (bins : EarleyBins T N (w.length + 1)) (binsIdx : Nat)
-    (hBins : binsIdx < w.length + 1) (binIdx : Nat) (hBin : binIdx < bins[binsIdx].length) :
-    Option (Tree T N) :=
-  let binItem := bins[binsIdx][binIdx]
-  match binItem.pointer with
+public partial def buildTree (G : ContextFreeGrammarList T N) (w : List T) (hw : ¬ w.isEmpty)
+    (bins : EarleyBins T N (w.length + 1)) (inv : isWellFormedBins G w bins) (k : Nat)
+    (hk : k < w.length + 1) (j : Nat) (hj : j < bins[k].length) : Option (Tree T N) :=
+  let binItem := bins[k][j]
+  match hp : binItem.pointer with
   | .null =>
     -- Start building a subtree
     some (Tree.node (Symbol.nonterminal binItem.item.rule.input) [])
   | .predecessor i => do
     -- Add sub tree starting from terminal
-    have : i < bins[binsIdx - 1].length := sorry -- sth about well-formed items
-    let t ← buildTree w bins (binsIdx-1) (by grind) i this
+    have : i < bins[k - 1].length := by grind
+    let t ← buildTree G w hw bins inv (k-1) (by grind) i this
     match t with
     | Tree.leaf d => none
     | Tree.node d ts =>
-      -- this is provable since the recursive call actually returned sth
-      have : w.length ≠ 0 := sorry
-      have : binsIdx - 1 < w.length := by omega
-      some (Tree.node d (ts.append [Tree.leaf (Symbol.terminal w[binsIdx-1])]))
+      have : k - 1 < w.length := by grind
+      some (Tree.node d (ts.append [Tree.leaf (Symbol.terminal w[k-1])]))
   | .reduction ps =>
     -- Add sub tree starting from non-terminal
-    match ps with
+    match hps : ps with
     | [] => none
-    -- TODO: Any reduction pointer is sufficient since we simply take one of the parse trees.
+    -- TODO: Any reduction pointer is sufficient since we simply take one of the parse trees?
     | ⟨endIdxA,i,j⟩ :: _ => do
-      have hEnd : endIdxA < w.length + 1 := sorry -- sth about well-formed items
-      have hi : i < bins[endIdxA].length := sorry -- sth about well-formed items
-      let t ← buildTree w bins endIdxA hEnd i hi
+      -- TODO: This is rather ugly. I should introduce a lemma to unfold WFPointers
+      --       if I know the item. Grind doesnt seem to be able to reason about reduction pointers
+      --       without simp/extra lemmas, that cannot be used by grind itself.
+      have hEnd : endIdxA < w.length + 1 := by
+        have ⟨_, pInv⟩:= inv k (by grind)
+        simp only [isWellFormedBinPointers, isWellFormedPointer, tsub_le_iff_right] at pInv
+        have := pInv binItem (by grind)
+        simp only [hp, List.mem_cons, forall_eq_or_imp] at this
+        grind
+      have hi : i < bins[endIdxA].length := by
+        have ⟨_, pInv⟩:= inv k (by grind)
+        simp only [isWellFormedBinPointers, isWellFormedPointer, tsub_le_iff_right] at pInv
+        have := pInv binItem (by grind)
+        simp only [hp, List.mem_cons, forall_eq_or_imp] at this
+        grind
+      let t ← buildTree G w hw bins inv endIdxA hEnd i hi
       match t with
       | Tree.leaf d => none
       | Tree.node d ts => do
-        have hj : j < bins[binsIdx].length := sorry
-        let t ← buildTree w bins binsIdx (by grind) j hj
+        have hj : j < bins[k].length := by
+          have ⟨_, pInv⟩:= inv k (by grind)
+          simp only [isWellFormedBinPointers, isWellFormedPointer, tsub_le_iff_right] at pInv
+          have := pInv binItem (by grind)
+          simp only [hp, List.mem_cons, forall_eq_or_imp] at this
+          grind
+        let t ← buildTree G w hw bins inv k (by grind) j hj
         some (Tree.node d (ts.append [t]))
 
 /--
@@ -121,14 +137,18 @@ Tries to parse a word with given grammar, and returns a parse tree if succesful.
 -/
 public def parse [LawfulBEq (EarleyItem T N)] (G : ContextFreeGrammarList T N) (w : List T) :
     Option (Tree T N) :=
-  let ⟨bins, inv⟩ := earleyList G w
-  -- Find the finished item, and follow its pointers.
-  match filterWithIdx bins[w.length]
-    (fun x => isFinished G.initial (w.map Symbol.terminal) x.item) with
-  | [] => none
-  -- TODO: This will be interesting to prove.
-  --       A lot about these indices being well-formed I'd imagine.
-  | (_, i)::_ => buildTree w bins w.length (by grind) i sorry
+  -- TODO: strictly speaking, this can be inferred from the result of earleyList
+  if hw : w.isEmpty then
+    none
+  else
+    let ⟨bins, inv⟩ := earleyList G w
+    -- Find the finished item, and follow its pointers.
+    let P := fun x => isFinished G.initial (w.map Symbol.terminal) x.item
+    match h : filterWithIdx bins[w.length] P with
+    | [] => none
+    | (_, i)::_ =>
+      have := filterWithIdx_le_length bins[w.length] P i (by grind)
+      buildTree G w hw bins inv w.length (by grind) i this
 
 end Parser
 end Earley
